
\newcommand{\implies}{\Longrightarrow}

\[
\beta = \frac{
\mathrm{P}(P, I)
}{
p
}
\]

\[
\mathrm{P} = \beta p
\]

\[
\alpha = \frac{
\mathrm{P}(\{ (P', I) \} \cap \{ (P', I), (P', I') \})
}{
\mathrm{P}(\{ (P', I), (P', I') \})
}
\]

\[
\alpha = \frac{
\mathrm{P}(P', I)
}{
1 - p
}
\]

\[
\mathrm{P}(P', I) = \alpha (1 - p)
\]

\[
\mathrm{P}(\{ (P, I) \} | \{ (P, I), (P', I) \})

\frac{
\mathrm{P}(P, I)
}{
\mathrm{P}(\{ (P, I), (P', I) \})
}

\frac{
\beta p
}{
\beta p + \alpha (1 - p)
}
\]

\[
\Omega _2 = \{ (\Omega _x, \Omega _y) : \forall \Omega _x, \Omega _y \subseteq \Omega \}

\mathrm{P}_2 (\{ (\Omega _x, \Omega _y) \}) = \mathrm{P}(\Omega _x) \cdot \mathrm{P}(\Omega _y) \forall \Omega _x, \Omega _y \in \Omega

% 20
= \mathrm{P}(
\{ ((P, i_1), (P', i_2)), ((P', i_3), (P, i_4)) : \forall i_1, i_2, i_3, i_4 \in \{ I, I' \} \} |
\{ ((x_1, I), (x_2, I)) : \forall x_1, x_2 \in \{ P, P' \} \}
)

% 21
= \frac{
\mathrm{P}_2 (
\{ ((P, i_1), (P', i_2)), ((P', i_3), (P, i_4)) : \forall i_1, i_2, i_3, i_4 \in \{ I, I' \} \} \cap \{ ((x_1, I), (x_2, I)) : \forall x_1, x_2 \in \{ P, P' \} \}
)
}{
\mathrm{P}_2(\{ ((x_1, I), (x_2, I)) : \forall x_1, x_2 \in \{ P, P' \} \})
}

% 21
= \frac{
\mathrm{P}_2 (
\{ ((P, I), (P', I))\}) + \mathrm{P}_2 ( \{ ((P', I), (P, I)) \}
)
}{
\mathrm{P}_2(\{ ((P, I), (P, I)), ((P', I), (P, I)), ((P, I), (P', I)), ((P', I), (P', I))\})
}

= \frac{
\mathrm{P}(P, I) \cdot \mathrm{P}(P', I) + \mathrm{P}(P', I) \cdot \mathrm{P}(P, I)
}{
\mathrm{P}(P, I)^2 + 2 \times \mathrm{P}(P, I) \cdot \mathrm{P}(P', I) + \mathrm{P}(P', I)^2
}

= \frac{
2 \times \beta p \cdot \alpha (1 - p)
}{
(\beta p)^2 + 2 \times \beta p \cdot \alpha (1 - p) + (\alpha (1 - p))^2
}

= \frac{
2 \alpha \beta p (1 - p)
}{
\alpha ^2 (1 - p)^2 + \beta ^2 p^2 + 2 \alpha \beta p (1 - p)
}
\]
